Generated/erc20shim/ERC20Shim/mapping_index_access_mapping_address_uint256_of_address_user.lean
@@ -34,6 +34,11 @@ lemma EVMAddrSize' {s : State} : (s, [Fin.shiftLeft 1 160]) = (s, [Address.size.
   simp
   exact shift_eq_size
 
+set_option maxHeartbeats 200000
+set_option maxRecDepth 800
+set_option pp.deepTerms true
+set_option pp.proofs true
+
 lemma mapping_index_access_mapping_address_uint256_of_address_abs_of_concrete {s₀ s₉ : State} {dataSlot slot key} :
   Spec (mapping_index_access_mapping_address_uint256_of_address_concrete_of_code.1 dataSlot slot key) s₀ s₉ →
   Spec (A_mapping_index_access_mapping_address_uint256_of_address dataSlot slot key) s₀ s₉ := by
@@ -42,33 +47,124 @@ lemma mapping_index_access_mapping_address_uint256_of_address_abs_of_concrete {s
   apply spec_eq
   intro hasFuel
   clr_funargs
-  sorry
+  
+  rw [ EVMSub', EVMShl', EVMAddrSize' ]; simp
+  rw [ Address.and_size_eq_ofUInt256 ]
+  rw [ multifill_cons, multifill_nil ]
+  simp
 
-  -- rw [ EVMSub', EVMShl', EVMAddrSize' ]; simp
-  -- rw [ Address.and_size_eq_ofUInt256 ]
-  -- rw [ multifill_cons, multifill_nil ]
-  -- simp
+  clr_varstore
 
-  -- clr_varstore
+  generalize acconut_def : Address.ofUInt256 key = account
+  intro code
+  unfold reviveJump at code
 
-  -- generalize acconut_def : Address.ofUInt256 key = account
-  -- intro prog address hasAddress
+  generalize prep_def : (mstore evm 0 ↑↑account).mstore 32 slot = state_prep at code
+  have Preserved_prep : Preserved evm state_prep := by
+    rw [← prep_def];
+    exact Preserved.trans mstore_preserved mstore_preserved
 
-  -- generalize prep_def : (mstore evm 0 ↑↑account).mstore 32 slot = state_prep
-  -- unfold keccak256 at prog
-  -- rw [ interval'_eq_interval 2 two_ne_zero (by norm_cast)
-  --    , mstore_mstore_of_ne, interval_of_mstore_eq_val_cons
-  --    , mstore_mstore_of_ne, zero_add, interval_of_mstore_eq_val_cons
-  --    , interval_of_0_eq_nil
-  --    ] at prog
-  -- unfold_let at prog
+  unfold keccak256 at code
+  unfold_let at code
+
+  split at code
+  -- some
+  case h_1 x h_lookup =>
+    right -- no hash collision
+    split at h_lookup
+    case h_1 val heq =>
+      rw [Option.some_inj] at h_lookup
+      -- lookup existing
+      rw [ interval'_eq_interval 2 two_ne_zero (by norm_cast)
+         , ← prep_def
+         , mstore_mstore_of_ne, interval_of_mstore_eq_val_cons
+         , mstore_mstore_of_ne, zero_add, interval_of_mstore_eq_val_cons
+         , interval_of_0_eq_nil
+         ] at heq
+      -- make sense of the code
+      rw [← h_lookup] at code
+      simp only [Fin.isValue, multifill_cons, multifill_nil'] at code
+      unfold setEvm State.insert State.lookup! at code
+      simp only [Fin.isValue, Finmap.lookup_insert, get!_some, isOk_Ok] at code
+      rw [← State.insert_of_ok] at code
+
+      rw [← code]
+      simp only [isOk_Ok, isOutOfFuel_insert', isOutOfFuel_Ok, not_false_eq_true, isOk_insert, evm_insert,
+  get_evm_of_ok, true_and]
+      split_ands
+
+      rw [preservesEvm_of_insert']
+      apply preservesEvm_of_preserved
+      simp [get_evm_of_ok]
+      exact Preserved_prep
+      use val, (prep_def ▸ heq)
+      simp only [insert_of_ok, store]
+
+    case h_2 val heq =>
+      split at h_lookup
+      swap; contradiction
+      rw [Option.some_inj] at h_lookup
+      
+      have : Finmap.lookup [account.val.cast, slot] state_prep.keccak_map = none := by
+        rw [ interval'_eq_interval 2 two_ne_zero (by norm_cast)
+           , ← prep_def
+           , mstore_mstore_of_ne, interval_of_mstore_eq_val_cons
+           , mstore_mstore_of_ne, zero_add, interval_of_mstore_eq_val_cons
+           , interval_of_0_eq_nil
+           ] at heq
+        exact (prep_def ▸ heq)
+      have int_ne_mem_map : [↑↑account, slot] ∉ state_prep.keccak_map := sorry
+
+      simp at code
+      unfold setEvm State.insert State.lookup! at code
+      simp at code
+      simp only [← h_lookup, ← State.insert_of_ok] at code
+      rw [← code]
+
+      split_ands
+      rw [preservesEvm_of_insert']
+      apply preservesEvm_of_preserved
+      simp [get_evm_of_ok]
+      apply Preserved.trans Preserved_prep
+    
+      -- obtain ⟨res, σ'⟩ := x
+      -- injection h_lookup with res_eq σ'_eq
+      exact Preserved_of_updated_keccak_map (σ := state_prep) rfl
+      done
+    done
+
+  case h_2 x h_lookup =>
+    split at h_lookup
+    done
+
+  -- -- generalize interval_def : List.map (Nat.toUInt256 ∘ UInt256.fromBytes!)
+  -- --                 (List.toChunks 32
+  -- --                 (mkInterval' state_prep.machine_state.memory 0 64)) = interval at code
+
+  -- -- have interval_eq : interval = mkInterval state_prep.machine_state.memory 0 2 := by sorry
+
+  -- -- have : List.map (Nat.toUInt256 ∘ UInt256.fromBytes!)
+  -- --                 (List.toChunks 32
+  -- --                 (mkInterval' state_prep.machine_state.memory 0 64)) =
+  -- --   mkInterval state_prep.machine_state.memory 0 2 := by sorry
+  -- split at code
+  -- next x h_lookup =>
+  --   split at h_lookup
+  --   done
+
+  -- simp_rw [ interval'_eq_interval 2 two_ne_zero (by sorry)
+  --    -- , mstore_mstore_of_ne, interval_of_mstore_eq_val_cons
+  --    -- , mstore_mstore_of_ne, zero_add, interval_of_mstore_eq_val_cons
+  --    -- , interval_of_0_eq_nil
+  --    ] at code
+
+  -- -- rw [ this ] at code
   -- rw [ mstore_preserves_keccak_map, mstore_preserves_keccak_map
   --    , hasAddress
-  --    ] at prog
+  --    ]
   -- simp at prog
   -- unfold setEvm State.insert State.lookup! at prog
   -- simp at prog
-
 
   -- rw [← prog]
   -- unfold State.lookup!
@@ -76,7 +172,7 @@ lemma mapping_index_access_mapping_address_uint256_of_address_abs_of_concrete {s
   -- apply And.intro
   -- · apply preservesEvm_eq
   --   simp
-  --   apply preserved_trans (e₁ := mstore evm 0 ↑↑account)
+  --   apply preserved_trans 
   --   · exact mstore_preserves
   --   · exact mstore_preserves
   -- · simp
